lazy_list/spec.v
@@ -4,6 +4,7 @@ From iris.heap_lang Require Import notation proofmode.
 From iris.base_logic.lib Require Export invariants.
 
 From SkipList.lazy_list Require Import code.
+From SkipList.lib Require Import misc lemmas.
 
 
 Local Open Scope Z.
@@ -15,108 +16,179 @@ Module LazyListSpec (Params: LAZYLIST_PARAMS).
   Section Proofs.
     Context `{!heapGS Σ} (N : namespace).
 
-    Definition oloc_to_val (ol: option loc) : val := 
-      match ol with
-      | None => NONEV
-      | Some l => SOMEV #l
-      end.
-    
-
-    (* 
-    * The sequence of keys must be the same and
-    * the lock invariant must hold in all nodes.
-    *)
-    Fixpoint list_equiv (L: list Z) (node: val) : iProp Σ :=
+    Fixpoint list_equiv (L: list node_rep) : iProp Σ :=
       match L with
-      | nil =>    ∃ (t: loc) (m: bool) (l: val),
-                  ⌜ node = SOMEV #t ⌝
-                  ∗
-                  t ↦ (#INT_MAX, NONEV, #m, l)
-                  (* ∗
-                  is_lock γ l ??? *)
+      | nil => True
+      | pred :: succs => 
+        match succs with
+        | nil => ∃ (l: loc),
+                 ⌜ node_next pred = Some l ⌝
+                 ∗
+                 l ↦ rep_to_node tail
 
-      | h :: t => ∃ (np: loc) (n: option loc) (m: bool) (l: val),
-                  ⌜ node = SOMEV #np ⌝
-                  ∗
-                  np ↦ (#h, oloc_to_val n, #m, l)
-                  ∗
-                  (* is_lock γ l ???
-                  ∗ *)
-                  ▷list_equiv t (oloc_to_val n)
+        | succ :: t => ∃ (l: loc),
+                       ⌜ node_next pred = Some l ⌝
+                       ∗
+                       l ↦ rep_to_node succ
+                       ∗
+                       list_equiv succs
+        end
       end.
+
+    Lemma list_equiv_cons (rep: node_rep) (L: list node_rep) :
+      list_equiv (rep :: L) 
+        ⊢ list_equiv L ∗ (list_equiv L -∗ list_equiv (rep :: L))
+    .
+    Proof.
+      destruct L as [|n].
+      * iIntros "Hrep". iDestruct "Hrep" as (l) "(? & ? & ?)".
+        iSplit. done. iIntros. 
+        iExists l. iFrame.
+      * iIntros "Hrep". iDestruct "Hrep" as (l) "(? & ? & ?)".
+        iFrame. iIntros. 
+        iExists l. iFrame.
+    Qed.
+
+    Lemma list_equiv_split (pred succ: node_rep) (L L1 L2: list node_rep):
+      L ++ [tail] = L1 ++ [pred; succ] ++ L2 →
+      list_equiv L ⊢ ∃ (l: loc),
+                     ⌜ node_next pred = Some l ⌝
+                     ∗
+                     l ↦ (rep_to_node succ)
+                     ∗
+                     (⌜ node_next pred = Some l ⌝ ∗ l ↦ (rep_to_node succ) -∗ list_equiv L)
+    .
+    Proof.
+      revert L. induction L1 => L Heq.
+      + destruct L as [|curr L].
+        { exfalso. inversion Heq. }
+        inversion Heq as [[H0 Heq']]; subst.
+        destruct L as [| curr L].
+        - inversion Heq'; subst.
+          iIntros "Hpred". iDestruct "Hpred" as (t) "(Hsome & Hpt)".
+          iExists t. iFrame.
+          iIntros "Htail". iExists t. iFrame.
+        - inversion Heq'; subst.
+          iIntros "Hpred". iDestruct "Hpred" as (n) "(Hsome & Hpt & Hmatch)".
+          iExists n. iFrame.
+          iIntros "succ".
+          iExists n. iFrame.
+      + destruct L as [| curr L].
+        { 
+          exfalso. inversion Heq  as [[H0 Heq']]; subst. 
+          destruct L1; inversion Heq'.
+        }
+        inversion Heq  as [[H0 Heq']]; subst.
+        iIntros "Hlist".
+        iPoseProof (list_equiv_cons with "Hlist") as "(Hlist & Himp)".
+        iPoseProof (IHL1 with "Hlist") as "Hpred". { done. }
+        iDestruct "Hpred" as (l) "(Hsome & Hpt & Hmatch)".
+        iExists l. iFrame. iIntros "(Hsome & Hpt)".
+        iApply "Himp". iApply "Hmatch". iFrame. 
+    Qed.
     
     (* 
     * The invariant for the lazy list asserts that
     * the underlying set S is sorted and must contain
     * the same elements as S.
     *)
-    Definition lazy_list_inv (S: gset Z) (v: val) : iProp Σ := 
-      ∃ (L: list Z) (h: loc) (n: option loc) (m: bool) (l: val),
+    Definition lazy_list_inv (S: gset node_rep) (head: node_rep) : iProp Σ := 
+      ∃ (L: list node_rep),
       ⌜ Permutation L (elements S) ⌝
       ∗
-      ⌜ Sorted Z.lt ([INT_MIN] ++ L ++ [INT_MAX]) ⌝
+      ⌜ Sorted node_lt ([head] ++ L ++ [tail]) ⌝
       ∗
-      ⌜ v = #h ⌝
-      ∗
-      h ↦ (#INT_MIN, oloc_to_val n, #m, l)
-      (* ∗
-      is_lock γ l ??? *)
-      ∗
-      list_equiv L (oloc_to_val n)
+      list_equiv ([head] ++ L)
     .
 
     (* 
     * Asserts that v points to a heap cell that 
     * represents the set S as a lazy list.
     *)
-    Definition is_lazy_list (S: gset Z) (v: val) : iProp Σ := 
-      inv N (lazy_list_inv S v).
+    Definition is_lazy_list (S: gset node_rep) (head: node_rep) : iProp Σ := 
+      inv N (lazy_list_inv S head).
 
     Theorem new_spec :
       {{{ True }}}
         new #()
-      {{{ v, RET v; 
-        is_lazy_list ∅ v 
+      {{{ (rep: node_rep), RET rep_to_node rep; 
+        is_lazy_list ∅ rep 
       }}}.
     Proof.
-      iIntros (Φ) "_ HPost".
-      wp_lam.
-      wp_alloc t as "Ht"; wp_alloc h as "Hh".
-      iMod (inv_alloc N ⊤ (lazy_list_inv ∅ #h) with "[Hh Ht]") as "Hinv".
-      + iNext.
-        iExists nil, h, (Some t), false, dummy_lock.
-        iSplit. done. 
-        iSplit. simpl. auto using HMIN_MAX. 
-        iSplit. done.
-        iFrame. iExists t, false, dummy_lock. by iFrame.
-      + by iApply "HPost".
+      iIntros (Φ) "_ HΦ".
+      wp_lam. wp_alloc t as "Ht". wp_pures.
+      set (head := (INT_MIN, Some t, false, dummy_lock)).
+      rewrite (fold_rep_to_node head).
+      iMod (inv_alloc N ⊤ (lazy_list_inv ∅ head) with "[Ht]") as "Hinv".
+      + iNext. iExists nil.
+        iSplit. done. iSplit. simpl. 
+        assert (node_lt head tail) as Hlt.
+        { unfold node_lt; unfold node_key; simpl; apply HMIN_MAX. }
+        auto using Hlt. 
+        iExists t. by iFrame.
+      + by iApply "HΦ".
     Qed.
+    
+    Theorem find_spec (head curr pred succ: node_rep) (key: Z)
+      (S: gset node_rep) (L Li Lm Le: list node_rep) :
+      Permutation (elements S) L →
+      Sorted node_lt ([head] ++ L ++ [tail]) →
+      INT_MIN < key < INT_MAX →
+      node_key pred < key <= node_key succ →
+      Li ++ [curr] ++ Lm ++ [succ] ++ Le = [head] ++ L ++ [tail] →
+      (∃ (L1 L2: list node_rep), L1 ++ [pred; succ] ++ L2 = [head] ++ L ++ [tail]) →
+      {{{ 
+        is_lazy_list S head 
+        ∗
+        ⌜ node_key curr = INT_MIN ∨ curr ∈ S ⌝
+        ∗
+        ⌜ node_key curr < key ⌝
+      }}}
+      find (rep_to_node curr) #key
+      {{{ ocurr, RET ocurr;
+        is_lazy_list S head
+        ∗
+        ⌜ ocurr = SOMEV (rep_to_node succ) ⌝
+      }}}.
+    Proof.
+      intros Hperm Hsort Hrange Hkey Hsplit_sep Hsplit_join.
+      iIntros (Φ) "(#Hinv&Hcurr_range&Hcurr_key) HΦ".
+      wp_lam. wp_let. wp_lam. wp_pures.
+      destruct (node_next curr) as [l|] eqn:Hcurr_next; wp_pures.
+      + wp_bind (Load _).
+        iInv N as (L') "(>%Hperm' & >%Hsort' & Hlist')" "Hclose".
 
-    Theorem contains_spec (S: gset Z) (v: val) (key: Z) 
+        assert (L = L') as <-.
+        {
+          eapply node_rep_sorted_eq.
+          * inversion Hsort as [| ? ? H]; subst.
+            eapply node_rep_sorted_app in H. destruct H. done.
+          * inversion Hsort' as [| ? ? H]; subst.
+            eapply node_rep_sorted_app in H. destruct H. done.
+          * by rewrite -Hperm.
+        }
+
+        destruct Lm as [|ck' Lm].
+        - rewrite (list_equiv_split curr succ ([head] ++ L)); last first.
+          { simpl in *. by rewrite -Hsplit_sep. }
+
+          admit.
+        - admit.
+      + admit.
+    Admitted.
+
+    (* Theorem contains_spec (S: gset Z) (v: val) (key: Z) 
       (Hrange: INT_MIN < key < INT_MAX) :
       {{{ is_lazy_list S v }}}
         contains v #key
       {{{ b, RET b; 
         is_lazy_list S v
         ∗
-        ⌜ (b = #false ∧ ¬ key ∈ S)
+        ⌜ (b = #false ∧ key ∉ S)
         ∨
         (b = #true ∧ key ∈ S) ⌝
       }}}.
     Proof.
-      iIntros (Φ) "#HPre HPost".
-      wp_lam. wp_let. wp_bind (Load _).
-      iInv N as (L h on m l) "(HPerm & HSort & >% & Hh & Hlist)" "Hclose"; subst; simpl.
-      wp_load.
-      iMod ("Hclose" with "[HPerm HSort Hh Hlist]") as "_".
-      { iNext. iExists L, h, on, m, l. by iFrame. }
-      iModIntro. wp_let. try repeat (wp_lam; wp_pures).
-      destruct on as [n|] eqn:Hn; wp_match.
-      + wp_op; case_bool_decide as Heq; wp_if.
-        lia. clear Heq.
-        admit.
-      + iExFalso.
-        admit.
-    Admitted.
+    Admitted. *)
   End Proofs.
 End LazyListSpec.
