lib/lemmas.v
@@ -1,0 +1,79 @@
+From Coq Require Import Lia Sorting.Sorted.
+
+From iris.heap_lang Require Import proofmode.
+
+From SkipList.lazy_list Require Import code.
+
+
+Local Open Scope Z.
+
+Lemma node_lt_transitive :
+  forall x y z, node_lt x y -> node_lt y z -> node_lt x z
+.
+Proof.
+  intros x y z. unfold node_lt.
+  intros xy yz. lia.
+Qed.
+
+Lemma node_rep_sorted_eq (l l': list node_rep):
+  Sorted node_lt l →
+  Sorted node_lt l' →
+  Permutation l l' →
+  l = l'.
+Proof.
+  revert l'.
+  induction l.
+  - intros l' ?? ?%Permutation.Permutation_nil. subst. auto.
+  - intros l' Hsorted Hsorted' Hperm.
+    destruct l' as [| a' l'].
+    { symmetry in Hperm. apply Permutation.Permutation_nil in Hperm. congruence. } 
+    destruct_decide (decide (a = a')) as Hcase.
+    { intros; subst.  f_equal.
+      eapply IHl.
+      { eapply Sorted_inv; eauto. }
+      { eapply Sorted_inv; eauto. }
+      apply Permutation.Permutation_cons_inv in Hperm; eauto.
+    }
+    
+    exfalso. cut (node_key a < node_key a' ∧ node_key a' < node_key a); first lia.
+    split.
+    * apply Sorted_StronglySorted in Hsorted; last eauto with *.
+      inversion Hsorted as [| ??? Hall]; subst.
+      assert (List.In a' (a :: l)) as [|]; subst.
+      { apply elem_of_list_In. rewrite Hperm. by left. }
+      ** congruence. 
+      ** eapply List.Forall_forall in Hall; eauto.
+      ** unfold Relations_1.Transitive.
+         apply node_lt_transitive.
+    * apply Sorted_StronglySorted in Hsorted'; last eauto with *.
+      inversion Hsorted' as [| ??? Hall]; subst.
+      assert (List.In a (a' :: l')) as [|]; subst.
+      { apply elem_of_list_In. rewrite -Hperm. by left. }
+      ** congruence. 
+      ** eapply List.Forall_forall in Hall; eauto.
+      ** unfold Relations_1.Transitive.
+         apply node_lt_transitive.
+Qed.
+
+Lemma StronglySorted_app {A: Type} R (L1 L2: list A):
+  StronglySorted R (L1 ++ L2) →
+  StronglySorted R L1 ∧ StronglySorted R L2.
+Proof.
+  induction L1.
+  - rewrite //=; intros; intuition; econstructor.
+  - intros Hs.
+    inversion Hs; subst; eauto.
+    edestruct IHL1; eauto. split; auto.
+    econstructor; eauto.
+    apply list.Forall_forall. intros. eapply list.Forall_forall; eauto.
+    apply elem_of_list_In. apply in_or_app. left. apply elem_of_list_In; done.
+Qed.
+
+Lemma node_rep_sorted_app (L1 L2: list node_rep):
+  Sorted node_lt (L1 ++ L2) → Sorted node_lt L1 ∧ Sorted node_lt L2.
+Proof.
+  intros HS. apply Sorted_StronglySorted in HS; last eauto with *.
+  + apply StronglySorted_app in HS as (?&?); split; eauto using StronglySorted_Sorted.
+  + unfold Relations_1.Transitive.
+    apply node_lt_transitive.
+Qed.
