lib/misc.v
@@ -1,0 +1,8 @@
+From iris.heap_lang Require Import notation.
+
+
+Definition oloc_to_val (ol: option loc) : val := 
+  match ol with
+  | None => NONEV
+  | Some l => SOMEV #l
+  end.
